io/case-study/WebServer.fst
@@ -13,30 +13,31 @@ open Utils
 type req_handler (fl:erased tflag) =
   (client:file_descr) ->
   (req:Bytes.bytes) ->
-  (send:(res:Bytes.bytes -> MIO (resexn unit) fl (requires (fun h -> did_not_respond h /\ valid_http_response res))
+  (send:(res:Bytes.bytes -> MIO (resexn unit) mymst fl (requires (fun h -> did_not_respond h /\ valid_http_response res))
                                             (ensures (fun _ _ lt -> exists r. lt == [EWrite Prog (client,res) r] /\
                                                                   wrote_at_least_once_to client lt)))) ->
-  MIO (resexn unit) fl (requires (fun h -> valid_http_request req /\ did_not_respond h))
-                       (ensures (fun h r lt -> enforced_locally pi h lt /\
-                                             (wrote_at_least_once_to client lt \/ Inr? r)))
+  MIO (resexn unit) mymst fl
+    (requires (fun h -> valid_http_request req /\ did_not_respond h))
+    (ensures (fun h r lt -> enforced_locally pi h lt /\
+                          (wrote_at_least_once_to client lt \/ Inr? r)))
 
 let static_cmd
   (cmd : io_cmds)
   (arg : io_sig.args cmd) :
-  MIO (io_sig.res cmd arg) IOActions
+  MIO (io_sig.res cmd arg) mymst IOActions
     (requires (fun h -> io_pre cmd arg h))
     (ensures (fun h (r:io_sig.res cmd arg) lt ->
         lt == [convert_call_to_event Prog cmd arg r])) =
   static_cmd Prog cmd arg
 
-
-let sendError400 (fd:file_descr) : MIO unit IOActions
+#push-options "--compat_pre_core 1"
+let sendError400 (fd:file_descr) : MIO unit mymst IOActions
  (fun _ -> True) (fun _ _ lt -> exists res r. lt == [EWrite Prog (fd, res) r]) =
   let _ = static_cmd Write (fd,(Bytes.utf8_encode "HTTP/1.1 400\n")) in
   ()
 
 let get_req (fd:file_descr) :
-  MIO (resexn Bytes.bytes) IOActions (fun _ -> True) (fun h r lt -> exists limit r'. (Inl? r <==> Inl? r') /\ lt == [ERead Prog (fd, limit) r']) =
+  MIO (resexn Bytes.bytes) mymst IOActions (fun _ -> True) (fun h r lt -> exists limit r'. (Inl? r <==> Inl? r') /\ lt == [ERead Prog (fd, limit) r']) =
   let limit : unit -> UInt8.t = (fun () -> UInt8.uint_to_t 255) in
   match static_cmd Read (fd,limit ()) with
   | Inl (msg, _) -> Inl msg
@@ -46,7 +47,7 @@ let process_connection
   (client : file_descr) 
   (#fl:erased tflag)
   (req_handler : req_handler (IOActions + fl)) : 
-  MIO unit (IOActions+fl) (fun _ -> True)
+  MIO unit mymst (IOActions+fl) (fun _ -> True)
     (fun _ _ lt -> every_request_gets_a_response lt) =
   admit ();
   introduce forall h lthandler lt lt'. enforced_locally pi h lthandler /\ every_request_gets_a_response (lt @ lt') ==> every_request_gets_a_response (lt @ lthandler @ lt')
@@ -72,7 +73,7 @@ let rec process_connections
   (to_read : lfds) 
   (#fl:erased tflag)
   (req_handler : req_handler (IOActions + fl)) : 
-  MIO lfds (IOActions+fl) (fun _ -> True)
+  MIO lfds mymst (IOActions+fl) (fun _ -> True)
     (fun _ _ lt -> every_request_gets_a_response lt) =
   match clients with
   | [] -> []
@@ -88,7 +89,7 @@ let rec process_connections
     end
  
 let get_new_connection (socket : file_descr) :
-  MIO (option file_descr) IOActions (fun _ -> True)
+  MIO (option file_descr) mymst IOActions (fun _ -> True)
     (fun _ _ lt -> every_request_gets_a_response lt) =
   match static_cmd Select (([socket] <: lfds), ([] <: lfds), ([] <: lfds), 100uy) with
   | Inl (to_accept, _, _) ->
@@ -105,7 +106,7 @@ let handle_connections
   (clients:lfds)
   (#fl:erased tflag)
   (req_handler : req_handler (IOActions + fl)) : 
-  MIO lfds (fl+IOActions) (fun _ -> True)
+  MIO lfds mymst (fl+IOActions) (fun _ -> True)
     (fun _ _ lt -> every_request_gets_a_response lt) =
   match static_cmd Select (clients, ([] <: lfds), ([] <: lfds), 100uy) with
   | Inl (to_read, _, _) ->
@@ -118,7 +119,7 @@ let server_loop_body
   (#fl:erased tflag)
   (req_handler : req_handler (IOActions + fl))
   (clients : lfds) :
-  MIO lfds (fl+IOActions) (fun _ -> True)
+  MIO lfds mymst (fl+IOActions) (fun _ -> True)
     (fun _ _ lt -> every_request_gets_a_response lt) =
   let clients' = (match get_new_connection socket with
                  | None -> clients
@@ -132,7 +133,7 @@ let rec server_loop
   (#fl:erased tflag)
   (req_handler : req_handler (IOActions + fl))
   (clients : lfds) :
-  MIO unit (fl+IOActions) (fun _ -> True)
+  MIO unit mymst (fl+IOActions) (fun _ -> True)
     (fun _ _ lt -> every_request_gets_a_response lt) =
   if iterations_count = 0 then ()
   else begin
@@ -142,7 +143,7 @@ let rec server_loop
   end
 
 let create_basic_server (ip:string) (port:UInt8.t) (limit:UInt8.t) :
-  MIO (resexn file_descr) IOActions (fun _ -> True)
+  MIO (resexn file_descr) mymst IOActions (fun _ -> True)
     (fun _ _ lt -> every_request_gets_a_response lt) =
   match static_cmd Socket () with
   | Inl socket -> 
@@ -157,7 +158,7 @@ let webserver
   (#fl:erased tflag)
   (req_handler : req_handler (IOActions + fl)) 
   () :
-  MIO int (IOActions + fl)
+  MIO int mymst (IOActions + fl)
     (requires (fun h -> True))
     (ensures (fun h r lt -> every_request_gets_a_response lt)) =
   match create_basic_server "0.0.0.0" 81uy 5uy with
@@ -171,33 +172,37 @@ let webserver
 
 (** Compiling Web Server **)
 
-let check_send_pre : tree pck_dc = 
+let check_send_pre : tree (pck_dc mymst) = 
   Node 
     (| Bytes.bytes, unit, (fun res h _ _ ->
-      Utils.did_not_respond' h && valid_http_response res) |)
+      Utils.did_not_respond' h && valid_http_response res), (fun res s0 _ _ -> s0.waiting () && valid_http_response res && true) |)
     Leaf
     Leaf
 
-let export_send (#fl:erased tflag) : exportable ((res:Bytes.bytes -> MIO (resexn unit) fl (fun h -> did_not_respond h && valid_http_response res)
-                                            (fun _ _ lt -> exists fd r. lt == [EWrite Prog (fd,res) r] ))) fl Utils.pi check_send_pre =
+let export_send (#fl:erased tflag) : exportable ((res:Bytes.bytes -> MIO (resexn unit) mymst fl (fun h -> did_not_respond h && valid_http_response res)
+                                            (fun _ _ lt -> exists fd r. lt == [EWrite Prog (fd,res) r] ))) fl Utils.pi mymst check_send_pre =
   exportable_arrow_pre_post_args Bytes.bytes unit _ _ #() #()
 
 
-let check_handler_post : tree pck_dc =
-  Node (| file_descr, unit, (fun (client:file_descr) _ _ lt -> 
-      Utils.wrote_at_least_once_to' client lt) |)
+let check_handler_post : tree (pck_dc mymst) =
+  Node (| 
+    file_descr, 
+    unit, 
+    (fun client _ _ lt -> Utils.wrote_at_least_once_to' client lt),
+    (fun client s0 _ s1 -> s1.written client)
+    |)
     check_send_pre 
     Leaf
 
-instance import_request_handler (fl:erased tflag) : safe_importable (req_handler fl) fl Utils.pi check_handler_post = {
-  sityp = file_descr -> Bytes.bytes -> export_send.ityp -> MIOpi (resexn unit) fl Utils.pi;
-  c_sityp = interm_arrow3 fl Utils.pi file_descr Bytes.bytes export_send.ityp #export_send.c_ityp (resexn unit);
-  safe_import = (fun (wf:file_descr -> Bytes.bytes -> export_send.ityp -> MIOpi (resexn unit) fl Utils.pi) eff_dcs -> 
+instance import_request_handler (fl:erased tflag) : safe_importable (req_handler fl) fl Utils.pi mymst check_handler_post = {
+  ityp = file_descr -> Bytes.bytes -> export_send.ityp -> MIOpi (resexn unit) fl Utils.pi mymst;
+  c_ityp = interm_arrow3 fl Utils.pi mymst file_descr Bytes.bytes export_send.ityp #export_send.c_ityp (resexn unit);
+  safe_import = (fun (wf:file_descr -> Bytes.bytes -> export_send.ityp -> MIOpi (resexn unit) fl Utils.pi mymst) eff_dcs -> 
     let f' : req_handler fl = (fun (fd:file_descr) req send -> 
       let send' = export_send.export (left eff_dcs) send in
       let (| dc_pck, eff_dc |) = root eff_dcs in
       // fd here is 4
-      let (| h, eff_dc' |) = eff_dc fd in
+      let (| _, h, eff_dc' |) = eff_dc fd in
       Classical.forall_intro (lemma_suffixOf_append h);
       let r : resexn unit = wf fd req send' in
       Classical.forall_intro_2 (Classical.move_requires_2 (lemma_append_rev_inv_tail h));
@@ -209,6 +214,7 @@ instance import_request_handler (fl:erased tflag) : safe_importable (req_handler
 }
 
 let cs_int : src_interface = {
+  mst = mymst;
   pi = Utils.pi;
   phi = Utils.phi;
   ct = req_handler;
