io/case-study/Execute.fst
@@ -2,12 +2,13 @@ module Execute
 
 open FStar.All
 open Compiler.Model1
+open Utils
 
 let the_p #a : hist_post #event a = fun lt r -> True
 
 exception Something_went_really_bad
 
-let rec skip_partial_calls (tree: mio int { forall h. dm_mio_theta tree the_p h }) : ML int =
+let rec skip_partial_calls (tree: mio mymst int { forall h. dm_mio_theta tree the_p h }) : ML int =
   match tree with
   | Return y -> y
   | PartialCall pre k -> begin
@@ -24,11 +25,11 @@ let rec skip_partial_calls (tree: mio int { forall h. dm_mio_theta tree the_p h 
 
 open FStar.Tactics
 
-let cast_mio (wp : hist 'a) (t : dm_mio 'a wp) : (x : mio 'a { wp `hist_ord` dm_mio_theta x }) =
+let cast_mio (wp : hist 'a) (t : dm_mio mymst 'a wp) : (x : mio mymst 'a { wp `hist_ord` dm_mio_theta x }) =
   t
 
-let execute (w:unit -> MIO int AllActions (fun _ -> True) (fun _ _ _ -> True)) : ML int by (compute ()) =
-  let dm_tree : dm_gmio int AllActions trivial_hist = reify (w ()) in
-  let dm_tree' : dm_mio int trivial_hist = dm_tree in
-  let dm_tree2 : (x : mio int { trivial_hist `hist_ord` dm_mio_theta x }) = cast_mio trivial_hist dm_tree' in
+let execute (w:unit -> MIO int mymst AllActions (fun _ -> True) (fun _ _ _ -> True)) : ML int by (compute ()) =
+  let dm_tree : dm_gmio int mymst AllActions trivial_hist = reify (w ()) in
+  let dm_tree' : dm_mio mymst int trivial_hist = dm_tree in
+  let dm_tree2 : (x : mio mymst int { trivial_hist `hist_ord` dm_mio_theta x }) = cast_mio trivial_hist dm_tree' in
   skip_partial_calls dm_tree2
